pcuic/theories/PCUICExpandLets.v
@@ -40,7 +40,7 @@ Fixpoint trans (t : term) : term :=
   | tCoFix mfix idx =>
     let mfix' := List.map (map_def trans trans) mfix in
     tCoFix mfix' idx
-  | tPrim i => tPrim i
+  (* | tPrim i => tPrim i *)
   end.
 
 Notation trans_decl := (map_decl trans).
